TreeCodeConversion.thy
@@ -15,10 +15,11 @@ primrec compile_closure :: "closure \<Rightarrow> tclosure" where
 fun compile_stack :: "cframe list \<Rightarrow> tree_code_state" where
   "compile_stack [] = TS [] [] []"
 | "compile_stack (CApp1 cs e # s) = (case compile_stack s of 
-      TS vs envs cd \<Rightarrow> TS vs (map compile_closure cs # envs) (compile e (TApply # cd)))"
+      TS vs envs cd \<Rightarrow> 
+        TS vs (map compile_closure (latest_environment s) # envs) (compile e (TApply # cd)))"
 | "compile_stack (CApp2 c # s) = (case compile_stack s of 
       TS vs envs cd \<Rightarrow> TS (compile_closure c # vs) envs (TApply # cd))"
-| "compile_stack (CReturn # s) = compile_stack s"
+| "compile_stack (CReturn cs # s) = compile_stack s"
 
 primrec compile_state :: "closure_state \<Rightarrow> tree_code_state" where
   "compile_state (CSE s cs e) = (case compile_stack s of 
@@ -53,92 +54,105 @@ lemma [dest]: "compile_closure c = TLam env cd \<Longrightarrow>
     \<exists>t cs e. c = CLam t cs e \<and> env = map compile_closure cs \<and> cd = compile e []"
   by (induction c) simp_all
 
-primrec all_returnc :: "cframe list \<Rightarrow> bool" where
+lemma tc_latest_environment [simp]: "s @ CApp1 cs e # s' :\<^sub>c t \<rightarrow> t' \<Longrightarrow> cs = latest_environment s'"
+proof (induction s arbitrary: t)
+  case (Cons f s)
+  moreover from Cons(2) obtain tt where "s @ CApp1 cs e # s' :\<^sub>c tt \<rightarrow> t'" 
+    by (induction "(f # s) @ CApp1 cs e # s'" t t' rule: typecheck_cstack.induct) simp_all
+  ultimately show ?case by simp
+qed fastforce+
+
+fun all_returnc :: "cframe list \<Rightarrow> bool" where
   "all_returnc [] = True"
-| "all_returnc (r # rs) = (r = CReturn \<and> all_returnc rs)"
+| "all_returnc (CReturn cs # rs) = all_returnc rs"
+| "all_returnc (r # rs) = False"
 
 lemma compile_stack_to_lookup [simp]: "TS vs (env # envs) (TLookup x # cd) = compile_stack s \<Longrightarrow> 
   \<exists>sr cs s' cd'. s = sr @ CApp1 cs (DVar x) # s' \<and> all_returnc sr \<and> 
-    compile_stack s' = TS vs envs cd' \<and> env = map compile_closure cs \<and> cd = TApply # cd'"
+    compile_stack s' = TS vs envs cd' \<and> env = map compile_closure (latest_environment s') \<and> 
+      cd = TApply # cd'"
 proof (induction s rule: compile_stack.induct)
   case (2 cs e s)
   then obtain s' where TS: "compile_stack s = TS vs envs s'" by (cases "compile_stack s") simp_all 
   moreover with 2 have "e = DVar x" by auto
-  moreover from 2 TS have "env = map compile_closure cs" by simp
+  moreover from 2 TS have "env = map compile_closure (latest_environment s)" by simp
   moreover from 2 TS have "cd = TApply # s'" by auto
   ultimately show ?case by fastforce
 next
-  case (4 s)
+  case (4 cs' s)
   then obtain sr cs s' cd' where "s = sr @ CApp1 cs (DVar x) # s' \<and> all_returnc sr \<and> 
-    compile_stack s' = TS vs envs cd' \<and> env = map compile_closure cs \<and> cd = TApply # cd'" 
-      by fastforce
-  hence "CReturn # s = (CReturn # sr) @ CApp1 cs (DVar x) # s' \<and>
-    all_returnc (CReturn # sr) \<and> compile_stack s' = TS vs envs cd' \<and> 
-      env = map compile_closure cs \<and> cd = TApply # cd'" by simp
+    compile_stack s' = TS vs envs cd' \<and> env = map compile_closure (latest_environment s') \<and> 
+      cd = TApply # cd'" by fastforce
+  hence "CReturn cs' # s = (CReturn cs' # sr) @ CApp1 cs (DVar x) # s' \<and>
+    all_returnc (CReturn cs' # sr) \<and> compile_stack s' = TS vs envs cd' \<and> 
+      env = map compile_closure (latest_environment s') \<and> cd = TApply # cd'" by simp
   thus ?case by fastforce
 qed (simp_all split: tree_code_state.splits)
 
 lemma compile_stack_to_pushcon [simp]: "TS vs (env # envs) (TPushCon k # cd) = compile_stack s \<Longrightarrow> 
   \<exists>sr cs s' cd'. s = sr @ CApp1 cs (DConst k) # s' \<and> all_returnc sr \<and> 
-    compile_stack s' = TS vs envs cd' \<and> env = map compile_closure cs \<and> cd = TApply # cd'"
+    compile_stack s' = TS vs envs cd' \<and> env = map compile_closure (latest_environment s') \<and> 
+      cd = TApply # cd'"
 proof (induction s rule: compile_stack.induct)
   case (2 cs e s)
   then obtain s' where TS: "compile_stack s = TS vs envs s'" by (cases "compile_stack s") simp_all 
   moreover with 2 have "e = DConst k" by auto
-  moreover from 2 TS have "env = map compile_closure cs" by simp
+  moreover from 2 TS have "env = map compile_closure (latest_environment s)" by simp
   moreover from 2 TS have "cd = TApply # s'" by auto
   ultimately show ?case by fastforce
 next
-  case (4 s)
+  case (4 cs' s)
   then obtain sr cs s' cd' where "s = sr @ CApp1 cs (DConst k) # s' \<and> all_returnc sr \<and> 
-    compile_stack s' = TS vs envs cd' \<and> env = map compile_closure cs \<and> cd = TApply # cd'" 
-      by fastforce
-  hence "CReturn # s = (CReturn # sr) @ CApp1 cs (DConst k) # s' \<and>
-    all_returnc (CReturn # sr) \<and> compile_stack s' = TS vs envs cd' \<and> 
-      env = map compile_closure cs \<and> cd = TApply # cd'" by simp
+    compile_stack s' = TS vs envs cd' \<and> env = map compile_closure (latest_environment s') \<and> 
+      cd = TApply # cd'" by fastforce
+  hence "CReturn cs' # s = (CReturn cs' # sr) @ CApp1 cs (DConst k) # s' \<and>
+    all_returnc (CReturn cs' # sr) \<and> compile_stack s' = TS vs envs cd' \<and> 
+      env = map compile_closure (latest_environment s') \<and> cd = TApply # cd'" by simp
   thus ?case by fastforce
 qed (simp_all split: tree_code_state.splits)
 
 lemma compile_stack_to_pushlam [simp]: "TS vs (env # envs) (TPushLam cd' # cd) = compile_stack s \<Longrightarrow> 
   \<exists>sr cs s' cd'' t e. s = sr @ CApp1 cs (DLam t e) # s' \<and> all_returnc sr \<and>  
-    compile_stack s' = TS vs envs cd'' \<and> env = map compile_closure cs \<and> cd = TApply # cd'' \<and> 
-      compile e [] = cd'"
+    compile_stack s' = TS vs envs cd'' \<and> env = map compile_closure (latest_environment s') \<and> 
+      cd = TApply # cd'' \<and> compile e [] = cd'"
 proof (induction s rule: compile_stack.induct)
   case (2 cs e s)
   then obtain s' where TS: "compile_stack s = TS vs envs s'" by (cases "compile_stack s") simp_all 
   moreover with 2 obtain t e' where "e = DLam t e' \<and> compile e' [] = cd'" by auto
-  moreover from 2 TS have "env = map compile_closure cs" by simp
+  moreover from 2 TS have "env = map compile_closure (latest_environment s)" by simp
   moreover from 2 TS have "cd = TApply # s'" by auto
   ultimately show ?case by fastforce
 next
-  case (4 s)
+  case (4 cs' s)
   then obtain sr cs s' cd'' t e' where "s = sr @ CApp1 cs (DLam t e') # s' \<and> all_returnc sr \<and> 
-    compile_stack s' = TS vs envs cd'' \<and> env = map compile_closure cs \<and> cd = TApply # cd'' \<and> 
-      compile e' [] = cd'" by fastforce
-  hence "CReturn # s = (CReturn # sr) @ CApp1 cs (DLam t e') # s' \<and>
-    all_returnc (CReturn # sr) \<and> compile_stack s' = TS vs envs cd'' \<and> 
-      env = map compile_closure cs \<and> cd = TApply # cd'' \<and> compile e' [] = cd'" by simp
+    compile_stack s' = TS vs envs cd'' \<and> env = map compile_closure (latest_environment s') \<and> 
+      cd = TApply # cd'' \<and> compile e' [] = cd'" by fastforce
+  hence "CReturn cs' # s = (CReturn cs' # sr) @ CApp1 cs (DLam t e') # s' \<and>
+    all_returnc (CReturn cs' # sr) \<and> compile_stack s' = TS vs envs cd'' \<and> 
+      env = map compile_closure  (latest_environment s') \<and> cd = TApply # cd'' \<and> compile e' [] = cd'" 
+    by simp
   thus ?case by fastforce
 qed (simp_all split: tree_code_state.splits)
 
 lemma compile_stack_to_enter [simp]: "TS vs (env # envs) (TEnter # cd) = compile_stack s \<Longrightarrow> 
   \<exists>sr s' cd' cs e\<^sub>1 e\<^sub>2. s = sr @ CApp1 cs (DApp e\<^sub>1 e\<^sub>2) # s' \<and> all_returnc sr \<and>  
-    compile_stack s' = TS vs envs cd' \<and> env = map compile_closure cs \<and> 
+    compile_stack s' = TS vs envs cd' \<and> env = map compile_closure (latest_environment s') \<and> 
       cd = compile e\<^sub>1 (compile e\<^sub>2 (TApply # TApply # cd'))" 
 proof (induction s rule: compile_stack.induct)
   case (2 cs e s)
-  then obtain cd' where TS: "compile_stack s = TS vs envs cd' \<and> env = map compile_closure cs \<and> 
-    TEnter # cd = compile e (TApply # cd')" by (cases "compile_stack s") simp_all
+  then obtain cd' where TS: "compile_stack s = TS vs envs cd' \<and> 
+    env = map compile_closure  (latest_environment s) \<and> TEnter # cd = compile e (TApply # cd')" 
+      by (cases "compile_stack s") simp_all
   moreover then obtain e\<^sub>1 e\<^sub>2 where "e = DApp e\<^sub>1 e\<^sub>2 \<and> 
     cd = compile e\<^sub>1 (compile e\<^sub>2 (TApply # TApply # cd'))" by fastforce
   ultimately show ?case by fastforce
 next
-  case (4 s)
+  case (4 cs' s)
   from 4 obtain sr s' cd' cs e\<^sub>1 e\<^sub>2 where "s = sr @ CApp1 cs (DApp e\<^sub>1 e\<^sub>2) # s' \<and> all_returnc sr \<and>
-    compile_stack s' = TS vs envs cd' \<and> env = map compile_closure cs \<and> 
+    compile_stack s' = TS vs envs cd' \<and> env = map compile_closure (latest_environment s') \<and> 
       cd = compile e\<^sub>1 (compile e\<^sub>2 (TApply # TApply # cd'))" by fastforce
-  moreover hence "CReturn # s = (CReturn # sr) @ CApp1 cs (DApp e\<^sub>1 e\<^sub>2) # s' \<and> 
-    all_returnc (CReturn # sr)" by simp
+  moreover hence "CReturn cs' # s = (CReturn cs' # sr) @ CApp1 cs (DApp e\<^sub>1 e\<^sub>2) # s' \<and> 
+    all_returnc (CReturn cs' # sr)" by simp
   ultimately show ?case by fastforce
 qed (simp_all split: tree_code_state.splits)
 
@@ -151,83 +165,93 @@ proof (induction s rule: compile_stack.induct)
     by (cases "compile_stack s") simp_all
   thus ?case by fastforce
 next
-  case (4 s)
+  case (4 cs' s)
   then obtain sr s' c vs' where "s = sr @ CApp2 c # s' \<and> all_returnc sr \<and> 
     compile_stack s' = TS vs' envs cd \<and> vs = compile_closure c # vs'" by fastforce
-  moreover hence "CReturn # s = (CReturn # sr) @ CApp2 c # s' \<and> 
-    all_returnc (CReturn # sr)" by simp
+  moreover hence "CReturn cs' # s = (CReturn cs' # sr) @ CApp2 c # s' \<and> 
+    all_returnc (CReturn cs' # sr)" by simp
   ultimately show ?case by fastforce
 qed (auto split: tree_code_state.splits)
 
-lemma compile_to_lookup [simp]: "TS vs (env # envs) (TLookup x # cd) = compile_state \<Sigma> \<Longrightarrow> 
-  (\<exists>s cs. compile_stack s = TS vs envs cd \<and> env = map compile_closure cs \<and> \<Sigma> = CSE s cs (DVar x)) \<or> 
-    (\<exists>sr s vs' c cs cd'. compile_stack s = TS vs' envs cd' \<and> env = map compile_closure cs \<and> 
-      all_returnc sr \<and> cd = TApply # cd' \<and> vs = compile_closure c # vs' \<and> 
-        \<Sigma> = CSC (sr @ CApp1 cs (DVar x) # s) c)"
-proof (induction \<Sigma>)
-  case (CSC s c)
+lemma compile_to_lookup [simp]: "\<Sigma> :\<^sub>c t \<Longrightarrow> 
+  TS vs (env # envs) (TLookup x # cd) = compile_state \<Sigma> \<Longrightarrow> 
+    (\<exists>s cs. compile_stack s = TS vs envs cd \<and> env = map compile_closure (latest_environment s) \<and> 
+      \<Sigma> = CSE s cs (DVar x)) \<or> (\<exists>sr s vs' c cs cd'. compile_stack s = TS vs' envs cd' \<and> 
+        env = map compile_closure (latest_environment s) \<and> all_returnc sr \<and> cd = TApply # cd' \<and> 
+          vs = compile_closure c # vs' \<and> \<Sigma> = CSC (sr @ CApp1 cs (DVar x) # s) c)"
+proof (induction \<Sigma> t rule: typecheck_closure_state.induct)
+  case (tcc_state_ret s t' t c)
   then obtain vs' where "TS vs' (env # envs) (TLookup x # cd) = compile_stack s \<and> 
     vs = compile_closure c # vs'" by (simp split: tree_code_state.splits)
   thus ?case using compile_stack_to_lookup by metis
 qed (auto split: tree_code_state.splits)
 
-lemma compile_to_pushcon [simp]: "TS vs (env # envs) (TPushCon k # cd) = compile_state \<Sigma> \<Longrightarrow> 
-  (\<exists>s cs. compile_stack s = TS vs envs cd \<and> env = map compile_closure cs \<and> 
-    \<Sigma> = CSE s cs (DConst k)) \<or> (\<exists>sr s vs' c cs cd'. compile_stack s = TS vs' envs cd' \<and> 
-      env = map compile_closure cs \<and> all_returnc sr \<and> cd = TApply # cd' \<and> 
-        vs = compile_closure c # vs' \<and> \<Sigma> = CSC (sr @ CApp1 cs (DConst k) # s) c)"
-proof (induction \<Sigma>)
-  case (CSC s c)
+lemma compile_to_pushcon [simp]: "\<Sigma> :\<^sub>c t \<Longrightarrow> 
+  TS vs (env # envs) (TPushCon k # cd) = compile_state \<Sigma> \<Longrightarrow> 
+    (\<exists>s cs. compile_stack s = TS vs envs cd \<and> env = map compile_closure (latest_environment s) \<and> 
+      \<Sigma> = CSE s cs (DConst k)) \<or> (\<exists>sr s vs' c cs cd'. compile_stack s = TS vs' envs cd' \<and> 
+        env = map compile_closure (latest_environment s) \<and> all_returnc sr \<and> cd = TApply # cd' \<and> 
+          vs = compile_closure c # vs' \<and> \<Sigma> = CSC (sr @ CApp1 cs (DConst k) # s) c)"
+proof (induction \<Sigma> t rule: typecheck_closure_state.induct)
+  case (tcc_state_ret s t' t c)
   then obtain vs' where "TS vs' (env # envs) (TPushCon k # cd) = compile_stack s \<and> 
     vs = compile_closure c # vs'" by (simp split: tree_code_state.splits)
   thus ?case using compile_stack_to_pushcon by metis
 qed (auto split: tree_code_state.splits)
 
-lemma compile_to_pushlam [simp]: "TS vs (env # envs) (TPushLam cd' # cd) = compile_state \<Sigma> \<Longrightarrow> 
-  (\<exists>s cs t e. compile_stack s = TS vs envs cd \<and> env = map compile_closure cs \<and> cd' = compile e [] \<and> 
-    \<Sigma> = CSE s cs (DLam t e)) \<or> (\<exists>sr s vs' c cd'' cs t e. compile_stack s = TS vs' envs cd'' \<and> 
-      cd = TApply # cd'' \<and> vs = compile_closure c # vs' \<and> env = map compile_closure cs \<and> 
-        cd' = compile e [] \<and> all_returnc sr \<and> \<Sigma> = CSC (sr @ CApp1 cs (DLam t e) # s) c)"
-proof (induction \<Sigma>)
-  case (CSC s c)
+lemma compile_to_pushlam [simp]: "\<Sigma> :\<^sub>c t \<Longrightarrow> 
+  TS vs (env # envs) (TPushLam cd' # cd) = compile_state \<Sigma> \<Longrightarrow> 
+    (\<exists>s cs t e. compile_stack s = TS vs envs cd \<and> env = map compile_closure (latest_environment s) \<and> 
+      cd' = compile e [] \<and> \<Sigma> = CSE s cs (DLam t e)) \<or> (\<exists>sr s vs' c cd'' cs t e. 
+        compile_stack s = TS vs' envs cd'' \<and> cd = TApply # cd'' \<and> vs = compile_closure c # vs' \<and>
+          env = map compile_closure (latest_environment s) \<and> cd' = compile e [] \<and> all_returnc sr \<and> 
+            \<Sigma> = CSC (sr @ CApp1 cs (DLam t e) # s) c)"
+proof (induction \<Sigma> t rule: typecheck_closure_state.induct)
+  case (tcc_state_ret s t' t c)
   then obtain vs' where "TS vs' (env # envs) (TPushLam cd' # cd) = compile_stack s \<and> 
     vs = compile_closure c # vs'" by (simp split: tree_code_state.splits)
   thus ?case using compile_stack_to_pushlam by metis
 qed (auto split: tree_code_state.splits)
 
-lemma compile_to_enter [simp]: "TS vs (env # envs) (TEnter # cd) = compile_state \<Sigma> \<Longrightarrow> 
-  (\<exists>s cs e\<^sub>1 e\<^sub>2 cd'. \<Sigma> = CSE s cs (DApp e\<^sub>1 e\<^sub>2) \<and> compile_stack s = TS vs envs cd' \<and> 
-    env = map compile_closure cs \<and> cd = compile e\<^sub>1 (compile e\<^sub>2 (TApply # cd'))) \<or>
-      (\<exists>sr s c vs' cd' cs e\<^sub>1 e\<^sub>2. \<Sigma> = CSC (sr @ CApp1 cs (DApp e\<^sub>1 e\<^sub>2) # s) c \<and> 
-        vs = compile_closure c # vs' \<and> compile_stack s = TS vs' envs cd' \<and> all_returnc sr \<and>
-          env = map compile_closure cs \<and> cd = compile e\<^sub>1 (compile e\<^sub>2 (TApply # TApply # cd')))" 
-proof (induction \<Sigma>) 
-  case (CSC s c)
+lemma compile_to_enter [simp]: "\<Sigma> :\<^sub>c t \<Longrightarrow> 
+  TS vs (env # envs) (TEnter # cd) = compile_state \<Sigma> \<Longrightarrow> 
+    (\<exists>s cs e\<^sub>1 e\<^sub>2 cd'. \<Sigma> = CSE s cs (DApp e\<^sub>1 e\<^sub>2) \<and> compile_stack s = TS vs envs cd' \<and> 
+      env = map compile_closure cs \<and> cd = compile e\<^sub>1 (compile e\<^sub>2 (TApply # cd'))) \<or>
+        (\<exists>sr s c vs' cd' cs e\<^sub>1 e\<^sub>2. \<Sigma> = CSC (sr @ CApp1 cs (DApp e\<^sub>1 e\<^sub>2) # s) c \<and> 
+          vs = compile_closure c # vs' \<and> compile_stack s = TS vs' envs cd' \<and> all_returnc sr \<and>
+            env = map compile_closure cs \<and> cd = compile e\<^sub>1 (compile e\<^sub>2 (TApply # TApply # cd')))" 
+proof (induction \<Sigma> t rule: typecheck_closure_state.induct)
+  case (tcc_state_ret s t' t c)
   then obtain vs' where "vs = compile_closure c # vs' \<and> 
     compile_stack s = TS vs' (env # envs) (TEnter # cd)" by (simp split: tree_code_state.splits)
-  thus ?case using compile_stack_to_enter by metis
+  moreover then obtain sr s' cd' cs e\<^sub>1 e\<^sub>2 where "s = sr @ CApp1 cs (DApp e\<^sub>1 e\<^sub>2) # s' \<and> 
+    all_returnc sr \<and> compile_stack s' = TS vs' envs cd' \<and> 
+      env = map compile_closure (latest_environment s') \<and> 
+        cd = compile e\<^sub>1 (compile e\<^sub>2 (TApply # TApply # cd'))" using compile_stack_to_enter by metis
+  moreover with tcc_state_ret have "cs = latest_environment s'" by (metis tc_latest_environment)
+  ultimately show ?case by metis
 qed (auto split: tree_code_state.splits)
 
-lemma compile_to_apply [simp]: "TS vs envs (TApply # cd) = compile_state \<Sigma> \<Longrightarrow> 
+lemma compile_to_apply [simp]: "\<Sigma> :\<^sub>c t \<Longrightarrow> TS vs envs (TApply # cd) = compile_state \<Sigma> \<Longrightarrow> 
   \<exists>sr s c c' vs'. \<Sigma> = CSC (sr @ CApp2 c' # s) c \<and> all_returnc sr \<and> 
     vs = compile_closure c # compile_closure c' # vs' \<and> compile_stack s = TS vs' envs cd"
-proof (induction \<Sigma>)
-  case (CSC s c)
+proof (induction \<Sigma> t rule: typecheck_closure_state.induct)
+  case (tcc_state_ret s t' t c)
   then obtain vs' where "compile_stack s = TS vs' envs (TApply # cd) \<and> vs = compile_closure c # vs'"
     by (simp split: tree_code_state.splits)
   thus ?case by (metis compile_stack_to_apply)
 qed (auto split: tree_code_state.splits)
 
 lemma [simp]: "all_returnc rs \<Longrightarrow> iter (\<leadsto>\<^sub>c) (CSC (rs @ s) c) (CSC s c)"
-proof (induction rs)
-  case (Cons r rs)
+proof (induction rs rule: all_returnc.induct)
+  case (2 cs rs)
   hence "iter (\<leadsto>\<^sub>c) (CSC (rs @ s) c) (CSC s c)" by simp
-  moreover have "CSC (CReturn # rs @ s) c \<leadsto>\<^sub>c CSC (rs @ s) c" by simp
-  ultimately have "iter (\<leadsto>\<^sub>c) (CSC (CReturn # rs @ s) c) (CSC s c)" by (metis iter_step)
+  moreover have "CSC (CReturn cs # rs @ s) c \<leadsto>\<^sub>c CSC (rs @ s) c" by simp
+  ultimately have "iter (\<leadsto>\<^sub>c) (CSC (CReturn cs # rs @ s) c) (CSC s c)" by (metis iter_step)
   with Cons show ?case by simp
 qed simp_all
 
-theorem correctt [simp]: "compile_state \<Sigma>\<^sub>c \<leadsto>\<^sub>t \<Sigma>\<^sub>t' \<Longrightarrow> 
+theorem correctt [simp]: "compile_state \<Sigma>\<^sub>c \<leadsto>\<^sub>t \<Sigma>\<^sub>t' \<Longrightarrow> \<Sigma>\<^sub>c :\<^sub>c t \<Longrightarrow>
   \<exists>\<Sigma>\<^sub>c'. iter (\<leadsto>\<^sub>c) \<Sigma>\<^sub>c \<Sigma>\<^sub>c' \<and> \<Sigma>\<^sub>t' = compile_state \<Sigma>\<^sub>c'"
 proof (induction "compile_state \<Sigma>\<^sub>c" \<Sigma>\<^sub>t' rule: evalt.induct)
   case (evt_lookup env x v vs envs cd)
@@ -243,9 +267,11 @@ proof (induction "compile_state \<Sigma>\<^sub>c" \<Sigma>\<^sub>t' rule: evalt.
   next
     case (CSC s c)
     then obtain rs s' vs' cs cd' where C: "compile_stack s' = TS vs' envs cd' \<and> 
-      env = map compile_closure cs \<and> cd = TApply # cd' \<and> vs = compile_closure c # vs' \<and> 
-        s = rs @ CApp1 cs (DVar x) # s' \<and> all_returnc rs" using compile_to_lookup by blast
-    with CSC obtain c' where C': "lookup cs x = Some c' \<and> v = compile_closure c'" by fastforce
+      env = map compile_closure (latest_environment s') \<and> cd = TApply # cd' \<and> 
+        vs = compile_closure c # vs' \<and> s = rs @ CApp1 cs (DVar x) # s' \<and> all_returnc rs" 
+      using compile_to_lookup by blast
+    with CSC have "cs = latest_environment s'" by fastforce
+    with CSC C obtain c' where C': "lookup cs x = Some c' \<and> v = compile_closure c'" by fastforce
     hence "CSE (CApp2 c # s') cs (DVar x) \<leadsto>\<^sub>c CSC (CApp2 c # s') c'" by simp
     moreover have "CSC (CApp1 cs (DVar x) # s') c \<leadsto>\<^sub>c CSE (CApp2 c # s') cs (DVar x)" by simp
     moreover from C have "iter (\<leadsto>\<^sub>c) (CSC (rs @ CApp1 cs (DVar x) # s') c) 
@@ -269,8 +295,9 @@ next
   next
     case (CSC s c)
     then obtain rs s' vs' cs cd' where C: "compile_stack s' = TS vs' envs cd' \<and> 
-      env = map compile_closure cs \<and> cd = TApply # cd' \<and> vs = compile_closure c # vs' \<and> 
-        s = rs @ CApp1 cs (DConst k) # s' \<and> all_returnc rs" using compile_to_pushcon by blast
+      env = map compile_closure (latest_environment s') \<and> cd = TApply # cd' \<and> 
+        vs = compile_closure c # vs' \<and> s = rs @ CApp1 cs (DConst k) # s' \<and> all_returnc rs" 
+      using compile_to_pushcon by blast
     have "CSE (CApp2 c # s') cs (DConst k) \<leadsto>\<^sub>c CSC (CApp2 c # s') (CConst k)" by simp
     moreover have "CSC (CApp1 cs (DConst k) # s') c \<leadsto>\<^sub>c CSE (CApp2 c # s') cs (DConst k)" by simp
     moreover from C have "iter (\<leadsto>\<^sub>c) (CSC (rs @ CApp1 cs (DConst k) # s') c) 
@@ -296,17 +323,18 @@ next
   next
     case (CSC s c)
     then obtain rs s' vs' cd'' cs t e where E: "compile_stack s' = TS vs' envs cd'' \<and> 
-      cd = TApply # cd'' \<and> vs = compile_closure c # vs' \<and> env = map compile_closure cs \<and> 
-        cd' = compile e [] \<and> s = rs @ CApp1 cs (DLam t e) # s' \<and> all_returnc rs" 
-          using compile_to_pushlam by blast
+      cd = TApply # cd'' \<and> vs = compile_closure c # vs' \<and> 
+        env = map compile_closure (latest_environment s') \<and> cd' = compile e [] \<and>
+          s = rs @ CApp1 cs (DLam t e) # s' \<and> all_returnc rs" using compile_to_pushlam by fastforce
     have "CSE (CApp2 c # s') cs (DLam t e) \<leadsto>\<^sub>c CSC (CApp2 c # s') (CLam t cs e)" by simp
     moreover have "CSC (CApp1 cs (DLam t e) # s') c \<leadsto>\<^sub>c CSE (CApp2 c # s') cs (DLam t e)" by simp
     moreover from E have "iter (\<leadsto>\<^sub>c) (CSC (rs @ CApp1 cs (DLam t e) # s') c) 
       (CSC (CApp1 cs (DLam t e) # s') c)" by fastforce
-    ultimately have
+    ultimately have X:
       "iter (\<leadsto>\<^sub>c) (CSC (rs @ CApp1 cs (DLam t e) # s') c) (CSC (CApp2 c # s') (CLam t cs e))" 
-        by (metis iter_step iter_refl iter_append)
-    with E show ?case by fastforce
+      by (metis iter_step iter_refl iter_append)
+    from CSC E have "cs = latest_environment s'" using tc_latest_environment by blast
+    with E X show ?case by fastforce
   qed
 next
   case (evt_enter vs env envs cd)
@@ -314,12 +342,13 @@ next
   proof (induction \<Sigma>\<^sub>c)
     case (CSE s cs e)
     then obtain e\<^sub>1 e\<^sub>2 cd' where E: "e = DApp e\<^sub>1 e\<^sub>2 \<and> compile_stack s = TS vs envs cd' \<and> 
-      env = map compile_closure cs \<and> cd = compile e\<^sub>1 (compile e\<^sub>2 (TApply # cd'))" 
+      env = map compile_closure (latest_environment s) \<and> cd = compile e\<^sub>1 (compile e\<^sub>2 (TApply # cd'))" 
         using compile_to_enter by blast
     have "CSE s cs (DApp e\<^sub>1 e\<^sub>2) \<leadsto>\<^sub>c CSE (CApp1 cs e\<^sub>2 # s) cs e\<^sub>1" by simp
-    hence "iter (\<leadsto>\<^sub>c) (CSE s cs (DApp e\<^sub>1 e\<^sub>2)) (CSE (CApp1 cs e\<^sub>2 # s) cs e\<^sub>1)" 
+    hence X: "iter (\<leadsto>\<^sub>c) (CSE s cs (DApp e\<^sub>1 e\<^sub>2)) (CSE (CApp1 cs e\<^sub>2 # s) cs e\<^sub>1)" 
       by (metis iter_step iter_refl)
-    with E show ?case by fastforce
+    from CSE E have "cs = latest_environment s" using tc_latest_environment by blast
+    with E X show ?case by fastforce
   next
     case (CSC s c)
     then obtain rs s' vs' cd' cs e\<^sub>1 e\<^sub>2 where S: "s = rs @ CApp1 cs (DApp e\<^sub>1 e\<^sub>2) # s' \<and> 
@@ -331,26 +360,31 @@ next
       by simp
     moreover from S have "iter (\<leadsto>\<^sub>c) (CSC (rs @ CApp1 cs (DApp e\<^sub>1 e\<^sub>2) # s') c) 
       (CSC (CApp1 cs (DApp e\<^sub>1 e\<^sub>2) # s') c)" by fastforce
-    ultimately have "iter (\<leadsto>\<^sub>c) (CSC (rs @ CApp1 cs (DApp e\<^sub>1 e\<^sub>2) # s') c) 
+    ultimately have X: "iter (\<leadsto>\<^sub>c) (CSC (rs @ CApp1 cs (DApp e\<^sub>1 e\<^sub>2) # s') c) 
       (CSE (CApp1 cs e\<^sub>2 # CApp2 c # s') cs e\<^sub>1)" by (metis iter_step iter_refl iter_append)
-    with S show ?case by fastforce
+    from CSC S have "cs = latest_environment s'" using tc_latest_environment by blast
+    with S X show ?case by fastforce
   qed
 next
   case (evt_apply v env cd' vs envs cd)
+  hence "\<exists>rs s c c' vs'. \<Sigma>\<^sub>c = CSC (rs @ CApp2 c' # s) c \<and> all_returnc rs \<and> 
+    (v # TLam env cd' # vs) = compile_closure c # compile_closure c' # vs' \<and> 
+      compile_stack s = TS vs' envs cd" using compile_to_apply by blast
   then obtain rs s c c' where S: "\<Sigma>\<^sub>c = CSC (rs @ CApp2 c' # s) c \<and> v = compile_closure c \<and> 
     compile_closure c' = TLam env cd' \<and> compile_stack s = TS vs envs cd \<and> all_returnc rs" 
-      using compile_to_apply by fastforce
+      by fastforce
   then obtain t cs e where C: "c' = CLam t cs e \<and> env = map compile_closure cs \<and> cd' = compile e []" 
     by fastforce
-  have "CSC (CApp2 (CLam t cs e) # s) c \<leadsto>\<^sub>c CSE (CReturn # s) (c # cs) e" by simp
+  have "CSC (CApp2 (CLam t cs e) # s) c \<leadsto>\<^sub>c CSE (CReturn (c # cs) # s) (c # cs) e" by simp
   moreover from S have "iter (\<leadsto>\<^sub>c) (CSC (rs @ CApp2 (CLam t cs e) # s) c) 
     (CSC (CApp2 (CLam t cs e) # s) c)" by fastforce
-  ultimately have "iter (\<leadsto>\<^sub>c) (CSC (rs @ CApp2 (CLam t cs e) # s) c) (CSE (CReturn # s) (c # cs) e)" 
-    by (metis iter_step iter_refl iter_append)
+  ultimately have "iter (\<leadsto>\<^sub>c) (CSC (rs @ CApp2 (CLam t cs e) # s) c) 
+    (CSE (CReturn (c # cs) # s) (c # cs) e)" 
+      by (metis iter_step iter_refl iter_append)
   with S C show ?case by fastforce
 qed
 
-theorem completet [simp]: "\<Sigma> \<leadsto>\<^sub>c \<Sigma>' \<Longrightarrow> iter (\<leadsto>\<^sub>t) (compile_state \<Sigma>) (compile_state \<Sigma>')"
+theorem completet [simp]: "\<Sigma> \<leadsto>\<^sub>c \<Sigma>' \<Longrightarrow> \<Sigma> :\<^sub>c t \<Longrightarrow> iter (\<leadsto>\<^sub>t) (compile_state \<Sigma>) (compile_state \<Sigma>')"
 proof (induction \<Sigma> \<Sigma>' rule: evalc.induct)
   case (evc_var cs x c s)
   obtain vs envs cd where S: "compile_stack s = TS vs envs cd" 
@@ -386,16 +420,18 @@ next
   have "TS vs (map compile_closure cs # envs) (TEnter # compile e\<^sub>1 (compile e\<^sub>2 (TApply # cd))) \<leadsto>\<^sub>t
       TS vs (map compile_closure cs # map compile_closure cs # envs) 
         (compile e\<^sub>1 (compile e\<^sub>2 (TApply # cd)))" by simp
-  hence "iter (\<leadsto>\<^sub>t) (TS vs (map compile_closure cs # envs) 
+  hence X: "iter (\<leadsto>\<^sub>t) (TS vs (map compile_closure cs # envs) 
     (TEnter # compile e\<^sub>1 (compile e\<^sub>2 (TApply # cd))))
       (TS vs (map compile_closure cs # map compile_closure cs # envs) 
         (compile e\<^sub>1 (compile e\<^sub>2 (TApply # cd))))" by (metis iter_step iter_refl)
-  with S show ?case by simp
+  from evc_app have "cs = latest_environment s" using tc_latest_environment by blast
+  with S X show ?case by simp
 next
   case (retc_app1 cs e\<^sub>2 s c\<^sub>1)
   obtain vs envs cd where "compile_stack s = TS vs envs cd" 
     by (induction s rule: compile_stack.induct) (simp_all split: tree_code_state.splits)
-  thus ?case by simp
+  moreover from retc_app1 have "cs = latest_environment s" using tc_latest_environment by blast
+  ultimately show ?case by simp
 next
   case (retc_app2 t cs e\<^sub>1 s c\<^sub>2)
   obtain vs envs cd where S: "compile_stack s = TS vs envs cd" 
@@ -411,10 +447,12 @@ next
   with S show ?case by simp
 qed simp_all
 
-lemma iter_completet [simp]: "iter (\<leadsto>\<^sub>c) \<Sigma> \<Sigma>' \<Longrightarrow> iter (\<leadsto>\<^sub>t) (compile_state \<Sigma>) (compile_state \<Sigma>')"
+lemma iter_completet [simp]: "iter (\<leadsto>\<^sub>c) \<Sigma> \<Sigma>' \<Longrightarrow> \<Sigma> :\<^sub>c t \<Longrightarrow>
+  iter (\<leadsto>\<^sub>t) (compile_state \<Sigma>) (compile_state \<Sigma>')"
 proof (induction \<Sigma> \<Sigma>' rule: iter.induct)
   case (iter_step \<Sigma> \<Sigma>' \<Sigma>'')
-  moreover hence "iter (\<leadsto>\<^sub>t) (compile_state \<Sigma>) (compile_state \<Sigma>')" by simp
+  hence "iter (\<leadsto>\<^sub>t) (compile_state \<Sigma>) (compile_state \<Sigma>')" by simp
+  moreover from iter_step have "iter (\<leadsto>\<^sub>t) (compile_state \<Sigma>') (compile_state \<Sigma>'')" by simp
   ultimately show ?case by (metis iter_append)
 qed simp_all
 
